new/proof/github_com/mit_pdos/tulip/tulip.v
@@ -1,0 +1,12 @@
+From New.proof Require Import github_com.mit_pdos.gokv.grove_ffi.
+
+From New.generatedproof.github_com.mit_pdos.tulip Require Import tulip.
+
+Section program.
+Context `{!heapGS Σ} `{!goGlobalsGS Σ}.
+
+#[global]
+Program Instance is_pkg_init_inst : IsPkgInit tulip :=
+  ltac2:(build_pkg_init ()).
+
+End program.
